src/Bedrock/Field/Synthesis/New/WordByWordMontgomery.v
@@ -334,6 +334,7 @@ Qed.
     valid_func (res mul_op _) ->
     forall functions,
       Cmd.spec_of_add_carryx (add_carryx:=Defaults.add_carryx)functions ->
+      Cmd.spec_of_sub_borrowx (sub_borrowx:=Defaults.sub_borrowx) functions ->
       spec_of_BinOp bin_mul ((Field.mul, mul_func) :: functions).
   Proof using M_eq check_args_ok mul_func_eq ok.
         (* tight_bounds_tighter_than. *)
@@ -369,6 +370,7 @@ Qed.
     valid_func (res square_op _) ->
     forall functions,
       Cmd.spec_of_add_carryx (add_carryx:=Defaults.add_carryx) functions ->
+      Cmd.spec_of_sub_borrowx (sub_borrowx:=Defaults.sub_borrowx) functions ->
       spec_of_UnOp un_square ((Field.square, square_func) :: functions).
   Proof using M_eq check_args_ok ok square_func_eq.
     intros. cbv [spec_of_UnOp un_square]. rewrite square_func_eq.
@@ -403,6 +405,7 @@ Qed.
     valid_func (res add_op _) ->
     forall functions,
       Cmd.spec_of_add_carryx (add_carryx:=Defaults.add_carryx) functions ->
+      Cmd.spec_of_sub_borrowx (sub_borrowx:=Defaults.sub_borrowx) functions ->
       spec_of_BinOp bin_add ((Field.add, add_func) :: functions).
   Proof using M_eq check_args_ok add_func_eq ok.
     intros. cbv [spec_of_BinOp bin_add]. rewrite add_func_eq.
@@ -437,6 +440,7 @@ Qed.
     valid_func (res sub_op _) ->
     forall functions,
       Cmd.spec_of_add_carryx (add_carryx:=Defaults.add_carryx) functions ->
+      Cmd.spec_of_sub_borrowx (sub_borrowx:=Defaults.sub_borrowx) functions ->
       spec_of_BinOp bin_sub ((Field.sub, sub_func) :: functions).
   Proof using M_eq check_args_ok sub_func_eq ok.
     intros. cbv [spec_of_BinOp bin_sub]. rewrite sub_func_eq.
@@ -470,6 +474,7 @@ Qed.
     valid_func (res opp_op _) ->
     forall functions,
       Cmd.spec_of_add_carryx (add_carryx:=Defaults.add_carryx) functions ->
+      Cmd.spec_of_sub_borrowx (sub_borrowx:=Defaults.sub_borrowx) functions ->
       spec_of_UnOp un_opp ((Field.opp, opp_func) :: functions).
   Proof using M_eq check_args_ok opp_func_eq ok.
     intros. cbv [spec_of_UnOp un_opp]. rewrite opp_func_eq.
@@ -504,6 +509,7 @@ Qed.
     valid_func (res from_bytes_op _) ->
     forall functions,
       Cmd.spec_of_add_carryx (add_carryx:=Defaults.add_carryx) functions ->
+      Cmd.spec_of_sub_borrowx (sub_borrowx:=Defaults.sub_borrowx) functions ->
       (@spec_of_from_bytes _ _ _ _ _ _ _ field_representation_raw) ((Field.from_bytes, from_bytes_func) :: functions).
   Proof using M_eq check_args_ok from_bytes_func_eq ok.
     intros. cbv [spec_of_from_bytes]. rewrite from_bytes_func_eq.
@@ -547,6 +553,7 @@ Qed.
     valid_func (res to_bytes_op _) ->
     forall functions,
       Cmd.spec_of_add_carryx (add_carryx:=Defaults.add_carryx) functions ->
+      Cmd.spec_of_sub_borrowx (sub_borrowx:=Defaults.sub_borrowx) functions ->
       (@spec_of_to_bytes _ _ _ _ _ _ _ field_representation_raw) ((Field.to_bytes, to_bytes_func) :: functions).
   Proof using M_eq check_args_ok ok to_bytes_func_eq.
     intros. cbv [spec_of_to_bytes]. rewrite to_bytes_func_eq.
@@ -627,6 +634,7 @@ Qed.
   valid_func (res from_mont_op _) ->
   forall functions,
       Cmd.spec_of_add_carryx (add_carryx:=Defaults.add_carryx) functions ->
+      Cmd.spec_of_sub_borrowx (sub_borrowx:=Defaults.sub_borrowx) functions ->
     (@spec_of_UnOp _ _ _ _ _ _ _ _ from_mont) un_from_mont ((from_mont, from_mont_func) :: functions).
     Proof using M_eq check_args_ok ok from_mont_func_eq.
     clear field_parameters_ok.
@@ -685,6 +693,7 @@ Qed.
   valid_func (res to_mont_op _) ->
   forall functions,
     Cmd.spec_of_add_carryx (add_carryx:=Defaults.add_carryx) functions ->
+    Cmd.spec_of_sub_borrowx (sub_borrowx:=Defaults.sub_borrowx) functions ->
     (@spec_of_UnOp _ _ _ _ _ _ _ _ to_mont) un_to_mont ((to_mont, to_mont_func) :: functions).
     Proof using M_eq check_args_ok ok to_mont_func_eq.
     intros. cbv [spec_of_UnOp un_to_mont]. rewrite to_mont_func_eq.
@@ -751,6 +760,7 @@ Qed.
   valid_func (res select_znz_op _) ->
   forall functions,
     Cmd.spec_of_add_carryx (add_carryx:=Defaults.add_carryx) functions ->
+    Cmd.spec_of_sub_borrowx (sub_borrowx:=Defaults.sub_borrowx) functions ->
     spec_of_selectznz ((select_znz, select_znz_func) :: functions).
 Proof using M_eq check_args_ok select_znz_func_eq ok.
   intros. cbv [spec_of_selectznz]. rewrite select_znz_func_eq.
